Bump to iris-dev, starting chan_* spec proofs

mutref.v
@@ -46,42 +46,63 @@ Class atomic_heap {Σ} `{!chanG Σ} := AtomicHeap {
 }.
 Global Arguments atomic_heap _ {_}.
 
-Section chanref.
+Definition expr := chan_lang.expr.
+
+(* Figure 16 *)
+Definition srv (r : expr) : val :=
+  rec: "loop" "v" :=
+    let: "dm" := recv r in
+    let: "reply" :=
+      λ: "m'" "v'",
+        Send (Fst "dm") "m'";; "loop" "v'" in
+    match: "m" with
+      NONE => "reply" "v" "v" (* GET *)
+    | SOME "w" =>
+        match: Snd "w" with
+            NONE => "reply" #() (Fst "w") (* SET *)
+          | SOME "v2" => "reply" (Fst "w") "v2" (* CAS *)
+      end
+    end.
+
+Definition rpc : val :=
+  λ: "r" "m",
+    let: "d" := newch in
+    Send "r" ("d", "m");; recv "d".
+
+Definition GET := NONE.
+Definition SET w:= SOME (w, NONE).
+Definition CAS v1 v2 := SOME (v1, SOME v2).
+
+Definition chan_get : val := λ: "e", rpc "e" GET.
+Definition chan_set : val := λ: "e" "e'", rpc "e" (SET "e'").
+Definition chan_cas : val := λ: "e" "e1" "e2", rpc "e" (CAS "e1" "e2").
+
+Definition chan_ref : val :=
+  λ: "e",
+    let: "r" := newch in
+    Fork (srv "r" "e");; "r".
+
+From iris Require Import proofmode.environments
+                         base_logic.lib.invariants.
+
+Section proof.
+
   Context `{!chanG Σ}.
+  Notation iProp := (iProp Σ).
 
-  Definition expr := chan_lang.expr.
+  Tactic Notation "wp_seq" := wp_pure (Rec BAnon BAnon _); wp_lam.
+  Lemma chan_get_spec (r : loc) (v : val):
+    ⊢ <<< ∀ w, r ↦ w >>> chan_set #r v @ ⊤ <<< r ↦ {[v]}, RET #() >>>.
+  Proof.
+    iIntros (Φ) "HΦ". iLöb as "IH".
+    wp_lam. wp_pures.
+    unfold rpc. wp_lam. wp_pures.
+    wp_bind (newch)%E.
+    iMod "HΦ" as (M) "[Hl [Hclose _]]".
+    iApply wp_newch; first by done.
+    iNext. iIntros (l) "H".
+    iMod ("Hclose" with "Hl") as "HΦ".
+    iModIntro. wp_pures.
+    (* awp_apply awp_send without "HΦ". *)
+  Admitted.
 
-  (* Figure 16 *)
-  Definition srv (r : expr) : val :=
-    rec: "loop" "v" :=
-      let: "dm" := recv r in
-      let: "reply" :=
-        λ: "m'" "v'",
-          Send (Fst "dm") "m'";; "loop" "v'" in
-      match: "m" with
-        NONE => "reply" "v" "v" (* GET *)
-      | SOME "w" =>
-          match: Snd "w" with
-              NONE => "reply" #() (Fst "w") (* SET *)
-            | SOME "v2" => "reply" (Fst "w") "v2" (* CAS *)
-        end
-      end.
-
-  Definition rpc : val :=
-    λ: "r" "m",
-      let: "d" := newch in
-      Send "r" ("d", "m");; recv "d".
-
-  Definition GET := NONE.
-  Definition SET w:= SOME (w, NONE).
-  Definition CAS v1 v2 := SOME (v1, SOME v2).
-
-  Definition chan_get e := rpc e GET.
-  Definition chan_set e e' := rpc e (SET e').
-  Definition chan_cas e e1 e2 := rpc e (CAS e1 e2).
-
-  Definition chan_ref : val :=
-    λ: "e",
-      let: "r" := newch in
-      Fork (srv "r" "e");; "r".
-End chanref.
