localchan.v
@@ -68,36 +68,6 @@ Section atomic_invariants.
     rewrite Heq. done.
   Qed.
 
-  Ltac wp_pures :=
-    iStartProof;
-    first [ (* The `;[]` makes sure that no side-condition magically spawns. *)
-            progress repeat (wp_pure _; [])
-          | wp_finish (* In case wp_pure never ran, make sure we do the usual cleanup. *)
-          ].
-
-  Ltac wp_apply_core lem tac_suc tac_fail := first
-    [iPoseProofCore lem as false (fun H =>
-      lazymatch goal with
-      | |- envs_entails _ (wp ?s ?E ?e ?Q) =>
-        reshape_expr e ltac:(fun K e' =>
-          wp_bind_core K; tac_suc H)
-      | |- envs_entails _ (twp ?s ?E ?e ?Q) =>
-        reshape_expr e ltac:(fun K e' =>
-          twp_bind_core K; tac_suc H)
-      | _ => fail 1 "wp_apply: not a 'wp'"
-      end)
-    |tac_fail ltac:(fun _ => wp_apply_core lem tac_suc tac_fail)
-    |let P := type of lem in
-    fail "wp_apply: cannot apply" lem ":" P ].
-
-  Tactic Notation "wp_apply" open_constr(lem) :=
-    wp_apply_core lem ltac:(fun H => iApplyHyp H; try iNext; try wp_expr_simpl)
-                      ltac:(fun cont => fail).
-  Tactic Notation "wp_smart_apply" open_constr(lem) :=
-    wp_apply_core lem ltac:(fun H => iApplyHyp H; try iNext; try wp_expr_simpl)
-                      ltac:(fun cont => wp_pure _; []; cont ()).
-
-
   Lemma awp_recv (c : loc) (m : val):
     ⊢ <<< ∀ (M : gset val), c ↦ M >>>
         recv (LitV $ LitLoc $ c) @ ⊤ <<< c ↦ (M ∖ {[m]}) ∧ ⌜m ∈ M⌝, RET m >>>.
